finished lindenbaum lemma except for the non-emptiness proof

src/natural_deduction.lean
@@ -27,6 +27,8 @@ inductive Deriv : set (Form vars) → Form vars → Prop
               → Deriv Γ C
 | Contra    : ∀ {Γ : set (Form vars)} {A : Form vars}, 
               Deriv (insert (~ A) Γ) ⊥ → Deriv Γ A
+| Weakening : ∀ {Γ Γ' : set (Form vars)} {A : Form vars},
+              (Γ ⊆ Γ') → (Deriv Γ A) → (Deriv Γ' A)
 
 open Deriv
 
@@ -53,6 +55,142 @@ begin
     apply Deriv.Ax,
     simp
   }
+end
+
+-- def compact_set [∀ (Γ : set (Form vars)) A, decidable (A ∈ Γ)] 
+--   : ∀ {Γ : set (Form vars)} {A}, (Γ ⊩ A) → set (Form vars)
+-- | Γ A (Deriv.Bottom_E h) := compact_set h
+-- | Γ A (Deriv.Ax _) := {A}
+-- | Γ (~ A) (Deriv.Not_I h) := if A ∈ Γ then compact_set h else compact_set h \ {A}
+-- | Γ ⊥ (Deriv.Not_E hnA hA) := compact_set hnA ∪ compact_set hA 
+-- | Γ (A ⋀ B) (Deriv.And_I hA hB) := compact_set hA ∪ compact_set hB 
+-- | Γ A (Deriv.And_E_1 hAB) := compact_set hAB 
+-- | Γ B (Deriv.And_E_2 hAB) := compact_set hAB
+-- | Γ (A ⋁ B) (Deriv.Or_I_1 hA) := compact_set hA
+-- | Γ (A ⋁ B) (Deriv.Or_I_2 hB) := compact_set hB
+-- | Γ C (Deriv.Or_E hAB hAC hBC) := sorry
+-- | Γ A (Deriv.Contra h) := if (~ A) ∈ Γ then compact_set h else compact_set h \ {~ A}
+-- using_well_founded {rel_tac := λ _ _, `[exact ⟨_, measure_wf psigma.snd.snd⟩]}
+
+def deriv_compactness [∀ (Γ : set (Form vars)) A, decidable (A ∈ Γ)] 
+{Γ : set (Form vars)} {A} (h : Γ ⊩ A) 
+  : ∃ Γ', Γ' ⊆ Γ ∧ Γ'.finite ∧ (Γ' ⊩ A) :=
+begin
+  --use compact_set h,
+  induction h,
+  case Deriv.Bottom_E : Γ A _ ih {
+    rcases ih with ⟨Γ', hsub, hfin, hbot⟩,
+    use Γ', use hsub, use hfin,
+    use Deriv.Bottom_E hbot,
+  },
+  case Deriv.Ax : Γ A h {
+    use {A},
+    split, { simp, use h },
+    split, { simp },
+    { apply Deriv.Ax, simp }
+  },
+  case Deriv.Not_I : Γ A _ ih {
+    rcases ih with ⟨Γ', hsub, hfin, hbot⟩,
+    use Γ' \ {A}, -- we need to remove the assumption added by the Not_I rule
+    refine ⟨_, _, _⟩,
+    { simp, exact hsub },
+    { exact set.finite.subset hfin (set.diff_subset Γ' {A}) },
+    { apply Deriv.Not_I, simp, exact Deriv.Weakening (by simp : Γ' ⊆ insert A Γ') hbot }
+  },
+  case Deriv.Not_E : Γ A _ _ ihnA ihA {
+    rcases ihnA with ⟨ΓnA, hnAsub, hnAfin, hnA⟩,
+    rcases ihA with ⟨ΓA, hAsub, hAfin, hA⟩,
+    use ΓnA ∪ ΓA,
+    refine ⟨_, _, _⟩,
+    { simp [hnAsub, hAsub] },
+    { simp [hnAfin, hAfin] },
+    { apply Deriv.Not_E,
+      exact Deriv.Weakening (by simp) hnA,
+      exact Deriv.Weakening (by simp) hA },
+  },
+  case Deriv.And_I : Γ A B _ _ ihA ihB {
+    rcases ihA with ⟨ΓA, hAsub, hAfin, hA⟩,
+    rcases ihB with ⟨ΓB, hBsub, hBfin, hB⟩,
+    use ΓA ∪ ΓB,
+    refine ⟨_, _, _⟩,
+    { simp [hAsub, hBsub] },
+    { simp [hAfin, hBfin] },
+    { apply Deriv.And_I,
+      exact Deriv.Weakening (by simp) hA,
+      exact Deriv.Weakening (by simp) hB },
+  },
+  case Deriv.And_E_1 : Γ A B _ ih {
+    rcases ih with ⟨Γ', hsub, hfin, hA⟩,
+    use Γ', use hsub, use hfin,
+    use Deriv.And_E_1 hA
+  },
+  case Deriv.And_E_2 : Γ A B _ ih {
+    rcases ih with ⟨Γ', hsub, hfin, hB⟩,
+    use Γ', use hsub, use hfin,
+    use Deriv.And_E_2 hB
+  },
+  case Deriv.Or_I_1 : Γ A B _ ih {
+    rcases ih with ⟨Γ', hsub, hfin, hA⟩,
+    use Γ', use hsub, use hfin,
+    use Deriv.Or_I_1 hA
+  },
+  case Deriv.Or_I_2 : Γ A B _ ih {
+    rcases ih with ⟨Γ', hsub, hfin, hB⟩,
+    use Γ', use hsub, use hfin,
+    use Deriv.Or_I_2 hB
+  },
+  case Deriv.Or_E : Γ A B C _ _ _ ihAB ihAC ihBC {
+    rcases ihAB with ⟨ΓAB, hABsub, hABfin, hAB⟩,
+    rcases ihAC with ⟨ΓAC, hACsub, hACfin, hAC⟩,
+    rcases ihBC with ⟨ΓBC, hBCsub, hBCfin, hBC⟩,
+    -- all the assumptions used except for the ones added by the Or_E rule.
+    use ΓAB ∪ ((ΓAC \ {A}) ∪ (ΓBC \ {B})),
+    refine ⟨_, _, _⟩,
+    { simp, exact ⟨hABsub, hACsub, hBCsub⟩ },
+    { simp, 
+      exact ⟨hABfin, 
+             set.finite.subset hACfin (set.diff_subset ΓAC {A}), 
+             set.finite.subset hBCfin (set.diff_subset ΓBC {B})⟩ },
+    { apply Deriv.Or_E,
+      { exact Deriv.Weakening (set.subset_union_left _ _) hAB },
+      { rw [←set.union_insert, ←set.insert_union, set.insert_diff_singleton],
+        refine Deriv.Weakening _ hAC,
+        apply set.subset_union_of_subset_right,
+        apply set.subset_union_of_subset_left,
+        exact set.subset_insert A ΓAC },
+      { rw [←set.union_insert, ←set.union_insert, set.insert_diff_singleton],
+        refine Deriv.Weakening _ hBC,
+        apply set.subset_union_of_subset_right,
+        apply set.subset_union_of_subset_right,
+        exact set.subset_insert B ΓBC }
+    }
+  },
+  case Deriv.Contra : Γ A _ ih {
+    -- similar to Not_I
+    rcases ih with ⟨Γ', hsub, hfin, hbot⟩,
+    use Γ' \ {~ A},
+    refine ⟨_, _, _⟩,
+    { simp, exact hsub },
+    { exact set.finite.subset hfin (set.diff_subset Γ' {~ A}) },
+    { apply Deriv.Contra, 
+      simp, 
+      exact Deriv.Weakening (by simp : Γ' ⊆ insert (~ A) Γ') hbot }
+  },
+  case Deriv.Weakening : Γ SΓ A hsub _ ih {
+    rcases ih with ⟨Γ', hsub', hfin, hA⟩,
+    use Γ', use trans hsub' hsub, use hfin,
+    use hA
+  }
+end
+
+theorem deriv_compactness' [∀ (Γ : set (Form vars)) A, decidable (A ∈ Γ)] 
+{Γ : set (Form vars)} (hfincon : ∀ (Δ : set (Form vars)), Δ ⊆ Γ → Δ.finite → consistent Δ) 
+  : consistent Γ :=
+begin
+  have := mt deriv_compactness,
+  simp at this,
+  exact this hfincon,
+  exact _inst_1 -- not sure why it cannot resolve this typeclass
 end
 
 #lint
